examples/ProcTwoStInv.v
@@ -9,6 +9,8 @@ Require Import Eqdep ProofIrrelevance.
 
 Set Implicit Arguments.
 
+Open Scope fmap.
+
 Section Invariants.
   Variables addrSize lgDataBytes rfIdx: nat.
 
@@ -36,7 +38,8 @@ Section Invariants.
                 Expr ty (SyntaxKind (Bit 2)) -> (* opTy *)
                 Expr ty (SyntaxKind (Bit rfIdx)) -> (* dst *)
                 Expr ty (SyntaxKind (Bit addrSize)) -> (* addr *)
-                Expr ty (SyntaxKind (Data lgDataBytes)) -> (* val *)
+                Expr ty (SyntaxKind (Data lgDataBytes)) -> (* val1 *)
+                Expr ty (SyntaxKind (Data lgDataBytes)) -> (* val2 *)
                 Expr ty (SyntaxKind (Data lgDataBytes)) -> (* rawInst *)
                 Expr ty (SyntaxKind (Bit addrSize)) -> (* curPc *)
                 Expr ty (SyntaxKind (Bit addrSize)) -> (* nextPc *)
@@ -49,8 +52,8 @@ Section Invariants.
                         Expr ty (SyntaxKind (Bit rfIdx)))
     (d2eAddr: forall ty, fullType ty (SyntaxKind d2eElt) ->
                          Expr ty (SyntaxKind (Bit addrSize)))
-    (d2eVal: forall ty, fullType ty (SyntaxKind d2eElt) ->
-                        Expr ty (SyntaxKind (Data lgDataBytes)))
+    (d2eVal1 d2eVal2: forall ty, fullType ty (SyntaxKind d2eElt) ->
+                                 Expr ty (SyntaxKind (Data lgDataBytes)))
     (d2eRawInst: forall ty, fullType ty (SyntaxKind d2eElt) ->
                             Expr ty (SyntaxKind (Data lgDataBytes)))
     (d2eCurPc: forall ty, fullType ty (SyntaxKind d2eElt) ->
@@ -60,84 +63,158 @@ Section Invariants.
     (d2eEpoch: forall ty, fullType ty (SyntaxKind d2eElt) ->
                           Expr ty (SyntaxKind Bool)).
 
-  Hypotheses (Hd2eOpType: forall opType dst addr val rawInst curPc nextPc epoch,
-                 evalExpr (d2eOpType _ (evalExpr (d2ePack opType dst addr val rawInst curPc nextPc epoch))) = evalExpr opType)
-             (Hd2eDst: forall opType dst addr val rawInst curPc nextPc epoch,
-                 evalExpr (d2eDst _ (evalExpr (d2ePack opType dst addr val rawInst curPc nextPc epoch))) = evalExpr dst)
-             (Hd2eAddr: forall opType dst addr val rawInst curPc nextPc epoch,
-                 evalExpr (d2eAddr _ (evalExpr (d2ePack opType dst addr val rawInst curPc nextPc epoch))) = evalExpr addr)
-             (Hd2eVal: forall opType dst addr val rawInst curPc nextPc epoch,
-                 evalExpr (d2eVal _ (evalExpr (d2ePack opType dst addr val rawInst curPc nextPc epoch))) = evalExpr val)
-             (Hd2eRawInst: forall opType dst addr val rawInst curPc nextPc epoch,
-                 evalExpr (d2eRawInst _ (evalExpr (d2ePack opType dst addr val rawInst curPc nextPc epoch))) = evalExpr rawInst)
-             (Hd2eCurPc: forall opType dst addr val rawInst curPc nextPc epoch,
-                 evalExpr (d2eCurPc _ (evalExpr (d2ePack opType dst addr val rawInst curPc nextPc epoch))) = evalExpr curPc)
-             (Hd2eNextPc: forall opType dst addr val rawInst curPc nextPc epoch,
-                 evalExpr (d2eNextPc _ (evalExpr (d2ePack opType dst addr val rawInst curPc nextPc epoch))) = evalExpr nextPc)
-             (Hd2eEpoch: forall opType dst addr val rawInst curPc nextPc epoch,
-                 evalExpr (d2eEpoch _ (evalExpr (d2ePack opType dst addr val rawInst curPc nextPc epoch))) = evalExpr epoch).
-  
+  Hypotheses
+    (Hd2eOpType: forall opType dst addr val1 val2 rawInst curPc nextPc epoch,
+        evalExpr (d2eOpType _ (evalExpr (d2ePack opType dst addr val1 val2 rawInst curPc nextPc epoch))) = evalExpr opType)
+    (Hd2eDst: forall opType dst addr val1 val2 rawInst curPc nextPc epoch,
+        evalExpr (d2eDst _ (evalExpr (d2ePack opType dst addr val1 val2 rawInst curPc nextPc epoch))) = evalExpr dst)
+    (Hd2eAddr: forall opType dst addr val1 val2 rawInst curPc nextPc epoch,
+        evalExpr (d2eAddr _ (evalExpr (d2ePack opType dst addr val1 val2 rawInst curPc nextPc epoch))) = evalExpr addr)
+    (Hd2eVal1: forall opType dst addr val1 val2 rawInst curPc nextPc epoch,
+        evalExpr (d2eVal1 _ (evalExpr (d2ePack opType dst addr val1 val2 rawInst curPc nextPc epoch))) = evalExpr val1)
+    (Hd2eVal2: forall opType dst addr val1 val2 rawInst curPc nextPc epoch,
+        evalExpr (d2eVal2 _ (evalExpr (d2ePack opType dst addr val1 val2 rawInst curPc nextPc epoch))) = evalExpr val2)
+    (Hd2eRawInst: forall opType dst addr val1 val2 rawInst curPc nextPc epoch,
+        evalExpr (d2eRawInst _ (evalExpr (d2ePack opType dst addr val1 val2 rawInst curPc nextPc epoch))) = evalExpr rawInst)
+    (Hd2eCurPc: forall opType dst addr val1 val2 rawInst curPc nextPc epoch,
+        evalExpr (d2eCurPc _ (evalExpr (d2ePack opType dst addr val1 val2 rawInst curPc nextPc epoch))) = evalExpr curPc)
+    (Hd2eNextPc: forall opType dst addr val1 val2 rawInst curPc nextPc epoch,
+        evalExpr (d2eNextPc _ (evalExpr (d2ePack opType dst addr val1 val2 rawInst curPc nextPc epoch))) = evalExpr nextPc)
+    (Hd2eEpoch: forall opType dst addr val1 val2 rawInst curPc nextPc epoch,
+        evalExpr (d2eEpoch _ (evalExpr (d2ePack opType dst addr val1 val2 rawInst curPc nextPc epoch))) = evalExpr epoch).
+
+  Variable (e2wElt: Kind).
+  Variable (e2wPack:
+              forall ty,
+                Expr ty (SyntaxKind d2eElt) -> (* decInst *)
+                Expr ty (SyntaxKind (Data lgDataBytes)) -> (* execVal *)
+                Expr ty (SyntaxKind e2wElt)).
+  Variables
+    (e2wDecInst: forall ty, fullType ty (SyntaxKind e2wElt) ->
+                            Expr ty (SyntaxKind d2eElt))
+    (e2wVal: forall ty, fullType ty (SyntaxKind e2wElt) ->
+                        Expr ty (SyntaxKind (Data lgDataBytes))).
+
+  Hypotheses
+    (He2wDecInst: forall decInst val,
+        evalExpr (e2wDecInst _ (evalExpr (e2wPack decInst val))) = evalExpr decInst)
+    (He2wVal: forall decInst val,
+        evalExpr (e2wVal _ (evalExpr (e2wPack decInst val))) = evalExpr val).
 
   Definition p2stInl := projT1 (p2stInl getOptype getLdDst getLdAddr getLdSrc calcLdAddr
                                         getStAddr getStSrc calcStAddr getStVSrc
                                         getSrc1 getSrc2 getDst exec getNextPc predictNextPc
-                                        d2ePack d2eOpType d2eDst d2eAddr d2eVal
-                                        d2eRawInst d2eCurPc d2eNextPc d2eEpoch).
+                                        d2ePack d2eOpType d2eDst d2eAddr d2eVal1 d2eVal2
+                                        d2eRawInst d2eCurPc d2eNextPc d2eEpoch
+                                        e2wPack e2wDecInst e2wVal).
 
-  Definition p2st_pc_epochs_inv_body
-             (fepochv eepochv d2efullv e2dfullv stallv: fullType type (SyntaxKind Bool))
-             (pcv: fullType type (SyntaxKind (Bit addrSize)))
-             (d2eeltv stalledv: fullType type (SyntaxKind d2eElt)) :=
-    (fepochv = eepochv -> e2dfullv = false) /\ (e2dfullv = false -> fepochv = eepochv) /\
-    (fepochv <> eepochv -> e2dfullv = true) /\ (e2dfullv = true -> fepochv <> eepochv) /\
+  (** Now invariants are defined below *)
 
-    (e2dfullv = true -> d2efullv = true -> evalExpr (d2eEpoch _ d2eeltv) = fepochv) /\
-    (d2efullv = true -> evalExpr (d2eEpoch _ d2eeltv) = fepochv ->
-     evalExpr (d2eNextPc _ d2eeltv) = pcv) /\
-    (d2efullv = true -> evalExpr (d2eEpoch _ d2eeltv) = eepochv -> e2dfullv = false) /\
-
-    (stallv = true -> e2dfullv = false) /\
-
-    (stallv = true -> d2efullv = true ->
-     (evalExpr (d2eNextPc _ stalledv) = evalExpr (d2eCurPc _ d2eeltv) /\
-      evalExpr (d2eEpoch _ d2eeltv) = fepochv)) /\
-    (stallv = true -> d2efullv = false -> e2dfullv = false ->
-     evalExpr (d2eNextPc _ stalledv) = pcv).
-
-  Record p2st_pc_epochs_inv (o: RegsT) : Prop :=
-    { pcv0 : fullType type (SyntaxKind (Bit addrSize));
-      Hpcv0 : M.find "pc"%string o = Some (existT _ _ pcv0);
-      fepochv0 : fullType type (SyntaxKind Bool);
-      Hfepochv0 : M.find "fEpoch"%string o = Some (existT _ _ fepochv0);
-
+  Definition p2st_scoreboard_waw_inv_body
+             (d2efullv: fullType type (SyntaxKind Bool))
+             (d2eeltv: fullType type (SyntaxKind d2eElt))
+             (e2wfullv: fullType type (SyntaxKind Bool))
+             (e2weltv: fullType type (SyntaxKind e2wElt))
+             (stallv: fullType type (SyntaxKind Bool))
+             (stalledv: fullType type (SyntaxKind d2eElt))
+             (sbv: fullType type (SyntaxKind (Vector Bool rfIdx))) :=
+    (d2efullv = true ->
+     ((evalExpr (d2eOpType _ d2eeltv) = opLd ->
+       sbv (evalExpr (d2eDst _ d2eeltv)) = true) /\
+      (evalExpr (d2eOpType _ d2eeltv) = opNm ->
+       sbv (evalExpr (d2eDst _ d2eeltv)) = true))) /\
+    (e2wfullv = true ->
+     let decInst := evalExpr (e2wDecInst _ e2weltv) in
+     ((evalExpr (d2eOpType _ decInst) = opLd ->
+       sbv (evalExpr (d2eDst _ decInst)) = true) /\
+      (evalExpr (d2eOpType _ decInst) = opNm ->
+       sbv (evalExpr (d2eDst _ decInst)) = true))) /\
+    (stallv = true ->
+     ((evalExpr (d2eOpType _ stalledv) = opLd ->
+       sbv (evalExpr (d2eDst _ stalledv)) = true) /\
+      (evalExpr (d2eOpType _ stalledv) = opNm ->
+       sbv (evalExpr (d2eDst _ stalledv)) = true))) /\
+    (d2efullv = true -> e2wfullv = true ->
+     let decInst := evalExpr (e2wDecInst _ e2weltv) in
+     (evalExpr (d2eOpType _ d2eeltv) = opLd \/ evalExpr (d2eOpType _ d2eeltv) = opNm) ->
+     (evalExpr (d2eOpType _ decInst) = opLd \/ evalExpr (d2eOpType _ decInst) = opNm) ->
+     evalExpr (d2eDst _ d2eeltv) <> evalExpr (d2eDst _ decInst)) /\
+    (d2efullv = true -> stallv = true ->
+     (evalExpr (d2eOpType _ d2eeltv) = opLd \/ evalExpr (d2eOpType _ d2eeltv) = opNm) ->
+     (evalExpr (d2eOpType _ stalledv) = opLd \/ evalExpr (d2eOpType _ stalledv) = opNm) ->
+     evalExpr (d2eDst _ d2eeltv) <> evalExpr (d2eDst _ stalledv)) /\
+    (e2wfullv = true -> stallv = true ->
+     let decInst := evalExpr (e2wDecInst _ e2weltv) in
+     (evalExpr (d2eOpType _ decInst) = opLd \/ evalExpr (d2eOpType _ decInst) = opNm) ->
+     (evalExpr (d2eOpType _ stalledv) = opLd \/ evalExpr (d2eOpType _ stalledv) = opNm) ->
+     evalExpr (d2eDst _ decInst) <> evalExpr (d2eDst _ stalledv)).
+  
+  Record p2st_scoreboard_waw_inv (o: RegsT) : Prop :=
+    { sbv0 : fullType type (SyntaxKind (Vector Bool rfIdx));
+      Hsbv0 : M.find "sbFlags"%string o = Some (existT _ _ sbv0);
+      
       d2eeltv0 : fullType type (SyntaxKind d2eElt);
       Hd2eeltv0 : M.find "d2e"--"elt"%string o = Some (existT _ _ d2eeltv0);
       d2efullv0 : fullType type (SyntaxKind Bool);
       Hd2efullv0 : M.find "d2e"--"full"%string o = Some (existT _ _ d2efullv0);
 
-      (* NOTE: Don't remove e2dElt even if it's not used in the invariant body. *)
-      e2deltv0 : fullType type (SyntaxKind (e2dElt addrSize));
-      He2deltv0 : M.find "e2d"--"elt"%string o = Some (existT _ _ e2deltv0);
-      e2dfullv0 : fullType type (SyntaxKind Bool);
-      He2dfullv0 : M.find "e2d"--"full"%string o = Some (existT _ _ e2dfullv0);
+      e2weltv0 : fullType type (SyntaxKind e2wElt);
+      He2weltv0 : M.find "e2w"--"elt"%string o = Some (existT _ _ e2weltv0);
+      e2wfullv0 : fullType type (SyntaxKind Bool);
+      He2wfullv0 : M.find "e2w"--"full"%string o = Some (existT _ _ e2wfullv0);
 
       stallv0 : fullType type (SyntaxKind Bool);
       Hstallv0 : M.find "stall"%string o = Some (existT _ _ stallv0);
       stalledv0 : fullType type (SyntaxKind d2eElt);
       Hstalledv0 : M.find "stalled"%string o = Some (existT _ _ stalledv0);
 
-      eepochv0 : fullType type (SyntaxKind Bool);
-      Heepochv0 : M.find "eEpoch"%string o = Some (existT _ _ eepochv0);
-    
-      Hinv0 : p2st_pc_epochs_inv_body fepochv0 eepochv0 d2efullv0 e2dfullv0
-                                      stallv0 pcv0 d2eeltv0 stalledv0 }.
+      Hinv0 : p2st_scoreboard_waw_inv_body d2efullv0 d2eeltv0 e2wfullv0 e2weltv0
+                                           stallv0 stalledv0 sbv0 }.
+
+  (* NOTE: this invariant requires p2st_scoreboard_waw_inv *)
+  Definition p2st_raw_inv_body
+             (prevv nextv: fullType type (SyntaxKind Bool))
+             (preveltv nexteltv: fullType type (SyntaxKind d2eElt)) :=
+    prevv = true -> nextv = true ->
+    (evalExpr (d2eOpType _ nexteltv) = opLd \/ evalExpr (d2eOpType _ nexteltv) = opNm) ->
+    ((evalExpr (d2eOpType _ preveltv) = opSt ->
+      (evalExpr (d2eDst _ nexteltv) <> evalExpr (getStSrc _ (evalExpr (d2eRawInst _ preveltv))) /\
+       evalExpr (d2eDst _ nexteltv) <> evalExpr (getStVSrc _ (evalExpr (d2eRawInst _ preveltv))))) /\
+     (evalExpr (d2eOpType _ preveltv) = opLd ->
+      evalExpr (d2eDst _ nexteltv) <> evalExpr (getLdSrc _ (evalExpr (d2eRawInst _ preveltv)))) /\
+     (evalExpr (d2eOpType _ preveltv) = opTh ->
+      evalExpr (d2eDst _ nexteltv) <> evalExpr (getSrc1 _ (evalExpr (d2eRawInst _ preveltv)))) /\
+     (evalExpr (d2eOpType _ preveltv) = opNm ->
+      (evalExpr (d2eDst _ nexteltv) <> evalExpr (getSrc1 _ (evalExpr (d2eRawInst _ preveltv))) /\
+       evalExpr (d2eDst _ nexteltv) <> evalExpr (getSrc2 _ (evalExpr (d2eRawInst _ preveltv)))))).
+  
+  Record p2st_raw_inv (o: RegsT) : Prop :=
+    { d2eeltv1 : fullType type (SyntaxKind d2eElt);
+      Hd2eeltv1 : M.find "d2e"--"elt"%string o = Some (existT _ _ d2eeltv1);
+      d2efullv1 : fullType type (SyntaxKind Bool);
+      Hd2efullv1 : M.find "d2e"--"full"%string o = Some (existT _ _ d2efullv1);
+
+      e2weltv1 : fullType type (SyntaxKind e2wElt);
+      He2weltv1 : M.find "e2w"--"elt"%string o = Some (existT _ _ e2weltv1);
+      e2wfullv1 : fullType type (SyntaxKind Bool);
+      He2wfullv1 : M.find "e2w"--"full"%string o = Some (existT _ _ e2wfullv1);
+
+      stallv1 : fullType type (SyntaxKind Bool);
+      Hstallv1 : M.find "stall"%string o = Some (existT _ _ stallv1);
+      stalledv1 : fullType type (SyntaxKind d2eElt);
+      Hstalledv1 : M.find "stalled"%string o = Some (existT _ _ stalledv1);
+
+      Hd2einv1 : p2st_raw_inv_body d2efullv1 stallv1 d2eeltv1 stalledv1;
+      He2winv1 : p2st_raw_inv_body e2wfullv1 stallv1 (evalExpr (e2wDecInst _ e2weltv1)) stalledv1;
+      Hd2winv1 : p2st_raw_inv_body d2efullv1 e2wfullv1 d2eeltv1 (evalExpr (e2wDecInst _ e2weltv1))
+    }.
 
   (* NOTE: this invariant requires p2st_raw_inv *)
   Definition p2st_decode_inv_body
              (pgmv: fullType type (SyntaxKind (Vector (Data lgDataBytes) addrSize)))
              (rfv: fullType type (SyntaxKind (Vector (Data lgDataBytes) rfIdx)))
-             (d2efullv: fullType type (SyntaxKind Bool))
-             (d2eeltv: fullType type (SyntaxKind d2eElt)) :=
+             (d2eeltv: fullType type (SyntaxKind d2eElt))
+             (d2efullv: fullType type (SyntaxKind Bool)) :=
     d2efullv = true ->
     let rawInst := evalExpr (d2eRawInst _ d2eeltv) in
     (rawInst = pgmv (evalExpr (d2eCurPc _ d2eeltv)) /\
@@ -151,23 +228,34 @@ Section Invariants.
       evalExpr (d2eAddr _ d2eeltv) =
       evalExpr (calcStAddr _ (evalExpr (getStAddr _ rawInst))
                            (rfv (evalExpr (getStSrc _ rawInst)))) /\
-      evalExpr (d2eVal _ d2eeltv) = rfv (evalExpr (getStVSrc _ rawInst)))) /\
+      evalExpr (d2eVal1 _ d2eeltv) = rfv (evalExpr (getStVSrc _ rawInst)))) /\
     (evalExpr (d2eOpType _ d2eeltv) = opTh ->
-     evalExpr (d2eVal _ d2eeltv) = rfv (evalExpr (getSrc1 _ rawInst))).
+     evalExpr (d2eVal1 _ d2eeltv) = rfv (evalExpr (getSrc1 _ rawInst))) /\
+    (evalExpr (d2eOpType _ d2eeltv) = opNm ->
+     (evalExpr (d2eDst _ d2eeltv) = evalExpr (getDst _ rawInst) /\
+      evalExpr (d2eVal1 _ d2eeltv) = rfv (evalExpr (getSrc1 _ rawInst)) /\
+      evalExpr (d2eVal2 _ d2eeltv) = rfv (evalExpr (getSrc2 _ rawInst)))).
 
   Record p2st_decode_inv (o: RegsT) : Prop :=
-    { pgmv1 : fullType type (SyntaxKind (Vector (Data lgDataBytes) addrSize));
-      Hpgmv1 : M.find "pgm"%string o = Some (existT _ _ pgmv1);
+    { pgmv2 : fullType type (SyntaxKind (Vector (Data lgDataBytes) addrSize));
+      Hpgmv2 : M.find "pgm"%string o = Some (existT _ _ pgmv2);
 
-      rfv1 : fullType type (SyntaxKind (Vector (Data lgDataBytes) rfIdx));
-      Hrfv1 : M.find "rf"%string o = Some (existT _ _ rfv1);
+      rfv2 : fullType type (SyntaxKind (Vector (Data lgDataBytes) rfIdx));
+      Hrfv2 : M.find "rf"%string o = Some (existT _ _ rfv2);
 
-      d2eeltv1 : fullType type (SyntaxKind d2eElt);
-      Hd2eeltv1 : M.find "d2e"--"elt"%string o = Some (existT _ _ d2eeltv1);
-      d2efullv1 : fullType type (SyntaxKind Bool);
-      Hd2efullv1 : M.find "d2e"--"full"%string o = Some (existT _ _ d2efullv1);
+      d2eeltv2 : fullType type (SyntaxKind d2eElt);
+      Hd2eeltv2 : M.find "d2e"--"elt"%string o = Some (existT _ _ d2eeltv2);
+      d2efullv2 : fullType type (SyntaxKind Bool);
+      Hd2efullv2 : M.find "d2e"--"full"%string o = Some (existT _ _ d2efullv2);
 
-      Hinv1 : p2st_decode_inv_body pgmv1 rfv1 d2efullv1 d2eeltv1 }.
+      e2weltv2 : fullType type (SyntaxKind e2wElt);
+      He2weltv2 : M.find "e2w"--"elt"%string o = Some (existT _ _ e2weltv2);
+      e2wfullv2 : fullType type (SyntaxKind Bool);
+      He2wfullv2 : M.find "e2w"--"full"%string o = Some (existT _ _ e2wfullv2);
+
+      Hd2einv2 : p2st_decode_inv_body pgmv2 rfv2 d2eeltv2 d2efullv2;
+      He2winv2 : p2st_decode_inv_body pgmv2 rfv2 (evalExpr (e2wDecInst _ e2weltv2)) e2wfullv2
+    }.
 
   (* NOTE: this invariant requires p2st_decode_inv *)
   Definition p2st_stalled_inv_body
@@ -183,80 +271,178 @@ Section Invariants.
      evalExpr (d2eDst _ stalledv) = evalExpr (getLdDst _ rawInst)).
 
   Record p2st_stalled_inv (o: RegsT) : Prop :=
-    { pgmv2 : fullType type (SyntaxKind (Vector (Data lgDataBytes) addrSize));
-      Hpgmv2 : M.find "pgm"%string o = Some (existT _ _ pgmv2);
+    { pgmv3 : fullType type (SyntaxKind (Vector (Data lgDataBytes) addrSize));
+      Hpgmv3 : M.find "pgm"%string o = Some (existT _ _ pgmv3);
 
-      rfv2 : fullType type (SyntaxKind (Vector (Data lgDataBytes) rfIdx));
-      Hrfv2 : M.find "rf"%string o = Some (existT _ _ rfv2);
-
-      stallv2 : fullType type (SyntaxKind Bool);
-      Hstallv2 : M.find "stall"%string o = Some (existT _ _ stallv2);
-      stalledv2 : fullType type (SyntaxKind d2eElt);
-      Hstalledv2 : M.find "stalled"%string o = Some (existT _ _ stalledv2);
-
-      Hinv2 : p2st_decode_inv_body pgmv2 rfv2 stallv2 stalledv2 }.
-  
-  (* NOTE: this invariant requires p2st_scoreboard_inv *)
-  Definition p2st_raw_inv_body
-             (d2efullv stallv: fullType type (SyntaxKind Bool))
-             (d2eeltv stalledv: fullType type (SyntaxKind d2eElt)) :=
-    d2efullv = true -> stallv = true -> evalExpr (d2eOpType _ stalledv) = opLd ->
-    ((evalExpr (d2eOpType _ d2eeltv) = opSt ->
-      (evalExpr (d2eDst _ stalledv) <> evalExpr (getStSrc _ (evalExpr (d2eRawInst _ d2eeltv))) /\
-       evalExpr (d2eDst _ stalledv) <> evalExpr (getStVSrc _ (evalExpr (d2eRawInst _ d2eeltv))))) /\
-     (evalExpr (d2eOpType _ d2eeltv) = opLd ->
-      evalExpr (d2eDst _ stalledv) <> evalExpr (getLdSrc _ (evalExpr (d2eRawInst _ d2eeltv)))) /\
-     (evalExpr (d2eOpType _ d2eeltv) = opTh ->
-      evalExpr (d2eDst _ stalledv) <> evalExpr (getSrc1 _ (evalExpr (d2eRawInst _ d2eeltv))))).
-
-  Record p2st_raw_inv (o: RegsT) : Prop :=
-    { d2eeltv3 : fullType type (SyntaxKind d2eElt);
-      Hd2eeltv3 : M.find "d2e"--"elt"%string o = Some (existT _ _ d2eeltv3);
-      d2efullv3 : fullType type (SyntaxKind Bool);
-      Hd2efullv3 : M.find "d2e"--"full"%string o = Some (existT _ _ d2efullv3);
+      rfv3 : fullType type (SyntaxKind (Vector (Data lgDataBytes) rfIdx));
+      Hrfv3 : M.find "rf"%string o = Some (existT _ _ rfv3);
 
       stallv3 : fullType type (SyntaxKind Bool);
       Hstallv3 : M.find "stall"%string o = Some (existT _ _ stallv3);
       stalledv3 : fullType type (SyntaxKind d2eElt);
       Hstalledv3 : M.find "stalled"%string o = Some (existT _ _ stalledv3);
 
-      Hinv : p2st_raw_inv_body d2efullv3 stallv3 d2eeltv3 stalledv3 }.
+      Hinv3 : p2st_stalled_inv_body pgmv3 rfv3 stallv3 stalledv3 }.
 
-  Definition p2st_scoreboard_inv_body
-             (d2efullv stallv sbvv: fullType type (SyntaxKind Bool))
-             (sbv: fullType type (SyntaxKind (Bit rfIdx)))
-             (d2eeltv stalledv: fullType type (SyntaxKind d2eElt)) :=
-    stallv = true -> evalExpr (d2eOpType _ stalledv) = opLd ->
-    (sbvv = true /\ evalExpr (d2eDst _ stalledv) = sbv).
+  Definition p2st_exec_inv_body
+             (pcv: fullType type (SyntaxKind (Bit addrSize)))
+             (rfv: fullType type (SyntaxKind (Vector (Data lgDataBytes) rfIdx)))
+             (e2wfullv: fullType type (SyntaxKind Bool))
+             (e2weltv: fullType type (SyntaxKind e2wElt)) :=
+    e2wfullv = true ->
+    let d2eeltv := evalExpr (e2wDecInst _ e2weltv) in
+    let rawInst := evalExpr (d2eRawInst _ d2eeltv) in
+    evalExpr (d2eOpType _ d2eeltv) = opNm ->
+    evalExpr (e2wVal _ e2weltv) =
+    evalExpr (exec _ (rfv (evalExpr (getSrc1 _ rawInst))) (rfv (evalExpr (getSrc2 _ rawInst)))
+                   (evalExpr (d2eCurPc _ d2eeltv)) rawInst).
 
-  Record p2st_scoreboard_inv (o: RegsT) : Prop :=
-    { sbv4 : fullType type (SyntaxKind (Bit rfIdx));
-      Hsbv4 : M.find "idx"%string o = Some (existT _ _ sbv4);
-      sbvv4 : fullType type (SyntaxKind Bool);
-      Hsbvv4 : M.find "valid"%string o = Some (existT _ _ sbvv4);
+  Record p2st_exec_inv (o: RegsT) : Prop :=
+    { pcv4 : fullType type (SyntaxKind (Bit addrSize));
+      Hpcv4 : M.find "pc"%string o = Some (existT _ _ pcv4);
+      rfv4 : fullType type (SyntaxKind (Vector (Data lgDataBytes) rfIdx));
+      Hrfv4 : M.find "rf"%string o = Some (existT _ _ rfv4);
 
-      d2eeltv4 : fullType type (SyntaxKind d2eElt);
-      Hd2eeltv4 : M.find "d2e"--"elt"%string o = Some (existT _ _ d2eeltv4);
-      d2efullv4 : fullType type (SyntaxKind Bool);
-      Hd2efullv4 : M.find "d2e"--"full"%string o = Some (existT _ _ d2efullv4);
+      e2weltv4 : fullType type (SyntaxKind e2wElt);
+      He2weltv4 : M.find "e2w"--"elt"%string o = Some (existT _ _ e2weltv4);
+      e2wfullv4 : fullType type (SyntaxKind Bool);
+      He2wfullv4 : M.find "e2w"--"full"%string o = Some (existT _ _ e2wfullv4);
 
-      stallv4 : fullType type (SyntaxKind Bool);
-      Hstallv4 : M.find "stall"%string o = Some (existT _ _ stallv4);
-      stalledv4 : fullType type (SyntaxKind d2eElt);
-      Hstalledv4 : M.find "stalled"%string o = Some (existT _ _ stalledv4);
+      Hinv4 : p2st_exec_inv_body pcv4 rfv4 e2wfullv4 e2weltv4 }.
 
-      Hinv : p2st_scoreboard_inv_body d2efullv4 stallv4 sbvv4 sbv4 d2eeltv4 stalledv4 }.
+  Definition p2st_epochs_inv_body
+             (fepochv eepochv d2efullv e2wfullv e2dfullv stallv: fullType type (SyntaxKind Bool))
+             (pcv: fullType type (SyntaxKind (Bit addrSize)))
+             (d2eeltv: fullType type (SyntaxKind d2eElt))
+             (e2weltv: fullType type (SyntaxKind e2wElt))
+             (stalledv: fullType type (SyntaxKind d2eElt)) :=
+    (fepochv = eepochv -> e2dfullv = false) /\ (e2dfullv = false -> fepochv = eepochv) /\
+    (fepochv <> eepochv -> e2dfullv = true) /\ (e2dfullv = true -> fepochv <> eepochv) /\
 
-  Hint Unfold p2st_pc_epochs_inv_body p2st_decode_inv_body p2st_stalled_inv_body
-       p2st_raw_inv_body p2st_scoreboard_inv_body : InvDefs.
+    (* fepoch: e2d and {d2e, e2w} *)
+    (e2dfullv = true ->
+     ((d2efullv = true -> evalExpr (d2eEpoch _ d2eeltv) = fepochv) /\
+      (e2wfullv = true -> evalExpr (d2eEpoch _ (evalExpr (e2wDecInst _ e2weltv))) = fepochv))) /\
+    (d2efullv = true -> e2wfullv = true ->
+     evalExpr (d2eEpoch _ (evalExpr (e2wDecInst _ e2weltv))) = fepochv ->
+     evalExpr (d2eEpoch _ d2eeltv) = fepochv) /\
+     
+    (* e2d and stalled *)
+    (e2dfullv = true -> stallv = false) /\ (stallv = true -> e2dfullv = false) /\
+    (fepochv = eepochv -> stallv = true ->
+     ((d2efullv = true -> evalExpr (d2eEpoch _ d2eeltv) = fepochv) /\
+      (e2wfullv = true -> evalExpr (d2eEpoch _ (evalExpr (e2wDecInst _ e2weltv))) = fepochv))) /\
+
+    (* eepoch: e2d and {d2e, e2w} *)
+    (d2efullv = true -> evalExpr (d2eEpoch _ d2eeltv) = eepochv -> e2dfullv = false) /\
+    (e2wfullv = true -> evalExpr (d2eEpoch _ (evalExpr (e2wDecInst _ e2weltv))) = eepochv ->
+     e2dfullv = false).
+
+  Record p2st_epochs_inv (o: RegsT) : Prop :=
+    { pcv5 : fullType type (SyntaxKind (Bit addrSize));
+      Hpcv5 : M.find "pc"%string o = Some (existT _ _ pcv5);
+      fepochv5 : fullType type (SyntaxKind Bool);
+      Hfepochv5 : M.find "fEpoch"%string o = Some (existT _ _ fepochv5);
+
+      d2eeltv5 : fullType type (SyntaxKind d2eElt);
+      Hd2eeltv5 : M.find "d2e"--"elt"%string o = Some (existT _ _ d2eeltv5);
+      d2efullv5 : fullType type (SyntaxKind Bool);
+      Hd2efullv5 : M.find "d2e"--"full"%string o = Some (existT _ _ d2efullv5);
+
+      (* NOTE: Don't remove e2dElt even if it's not used in the invariant body. *)
+      e2deltv5 : fullType type (SyntaxKind (e2dElt addrSize));
+      He2deltv5 : M.find "e2d"--"elt"%string o = Some (existT _ _ e2deltv5);
+      e2dfullv5 : fullType type (SyntaxKind Bool);
+      He2dfullv5 : M.find "e2d"--"full"%string o = Some (existT _ _ e2dfullv5);
+
+      e2weltv5 : fullType type (SyntaxKind e2wElt);
+      He2weltv5 : M.find "e2w"--"elt"%string o = Some (existT _ _ e2weltv5);
+      e2wfullv5 : fullType type (SyntaxKind Bool);
+      He2wfullv5 : M.find "e2w"--"full"%string o = Some (existT _ _ e2wfullv5);
+
+      stallv5 : fullType type (SyntaxKind Bool);
+      Hstallv5 : M.find "stall"%string o = Some (existT _ _ stallv5);
+      stalledv5 : fullType type (SyntaxKind d2eElt);
+      Hstalledv5 : M.find "stalled"%string o = Some (existT _ _ stalledv5);
+
+      eepochv5 : fullType type (SyntaxKind Bool);
+      Heepochv5 : M.find "eEpoch"%string o = Some (existT _ _ eepochv5);
+      
+      Hinv5 : p2st_epochs_inv_body fepochv5 eepochv5 d2efullv5 e2wfullv5 e2dfullv5 stallv5
+                                   pcv5 d2eeltv5 e2weltv5 stalledv5 }.
+
+  Definition p2st_pc_inv_body
+             (fepochv eepochv d2efullv e2wfullv e2dfullv stallv: fullType type (SyntaxKind Bool))
+             (pcv: fullType type (SyntaxKind (Bit addrSize)))
+             (d2eeltv: fullType type (SyntaxKind d2eElt))
+             (e2weltv: fullType type (SyntaxKind e2wElt))
+             (stalledv: fullType type (SyntaxKind d2eElt)) :=
+    (* pc: d2e *)
+    (d2efullv = true -> evalExpr (d2eEpoch _ d2eeltv) = fepochv ->
+     evalExpr (d2eNextPc _ d2eeltv) = pcv) /\
+    (* pc: e2w *)
+    (e2wfullv = true ->
+     ((d2efullv = true ->
+       evalExpr (d2eEpoch _ (evalExpr (e2wDecInst _ e2weltv))) = evalExpr (d2eEpoch _ d2eeltv) ->
+       evalExpr (d2eNextPc _ (evalExpr (e2wDecInst _ e2weltv))) = evalExpr (d2eCurPc _ d2eeltv)) /\
+      (d2efullv = false ->
+       evalExpr (d2eEpoch _ (evalExpr (e2wDecInst _ e2weltv))) = fepochv ->
+       evalExpr (d2eNextPc _ (evalExpr (e2wDecInst _ e2weltv))) = pcv))) /\
+    (* pc: stalled *)
+    (stallv = true ->
+     ((e2wfullv = true -> evalExpr (d2eNextPc _ stalledv) =
+                          evalExpr (d2eCurPc _ (evalExpr (e2wDecInst _ e2weltv)))) /\
+      (e2wfullv = false -> d2efullv = true ->
+       evalExpr (d2eNextPc _ stalledv) = evalExpr (d2eCurPc _ d2eeltv)) /\
+      (e2wfullv = false -> d2efullv = false -> evalExpr (d2eNextPc _ stalledv) = pcv))).
+
+  Record p2st_pc_inv (o: RegsT) : Prop :=
+    { pcv6 : fullType type (SyntaxKind (Bit addrSize));
+      Hpcv6 : M.find "pc"%string o = Some (existT _ _ pcv6);
+      fepochv6 : fullType type (SyntaxKind Bool);
+      Hfepochv6 : M.find "fEpoch"%string o = Some (existT _ _ fepochv6);
+
+      d2eeltv6 : fullType type (SyntaxKind d2eElt);
+      Hd2eeltv6 : M.find "d2e"--"elt"%string o = Some (existT _ _ d2eeltv6);
+      d2efullv6 : fullType type (SyntaxKind Bool);
+      Hd2efullv6 : M.find "d2e"--"full"%string o = Some (existT _ _ d2efullv6);
+
+      (* NOTE: Don't remove e2dElt even if it's not used in the invariant body. *)
+      e2deltv6 : fullType type (SyntaxKind (e2dElt addrSize));
+      He2deltv6 : M.find "e2d"--"elt"%string o = Some (existT _ _ e2deltv6);
+      e2dfullv6 : fullType type (SyntaxKind Bool);
+      He2dfullv6 : M.find "e2d"--"full"%string o = Some (existT _ _ e2dfullv6);
+
+      e2weltv6 : fullType type (SyntaxKind e2wElt);
+      He2weltv6 : M.find "e2w"--"elt"%string o = Some (existT _ _ e2weltv6);
+      e2wfullv6 : fullType type (SyntaxKind Bool);
+      He2wfullv6 : M.find "e2w"--"full"%string o = Some (existT _ _ e2wfullv6);
+
+      stallv6 : fullType type (SyntaxKind Bool);
+      Hstallv6 : M.find "stall"%string o = Some (existT _ _ stallv6);
+      stalledv6 : fullType type (SyntaxKind d2eElt);
+      Hstalledv6 : M.find "stalled"%string o = Some (existT _ _ stalledv6);
+
+      eepochv6 : fullType type (SyntaxKind Bool);
+      Heepochv6 : M.find "eEpoch"%string o = Some (existT _ _ eepochv6);
+      
+      Hinv6 : p2st_pc_inv_body fepochv6 eepochv6 d2efullv6 e2wfullv6 e2dfullv6 stallv6
+                               pcv6 d2eeltv6 e2weltv6 stalledv6 }.
+
+  Hint Unfold p2st_scoreboard_waw_inv_body p2st_raw_inv_body
+       p2st_decode_inv_body p2st_stalled_inv_body
+       p2st_exec_inv_body p2st_epochs_inv_body
+       p2st_pc_inv_body : InvDefs.
 
   Ltac p2st_inv_old :=
     repeat match goal with
-           | [H: p2st_pc_epochs_inv _ |- _] => destruct H
+           | [H: p2st_scoreboard_waw_inv _ |- _] => destruct H
+           | [H: p2st_raw_inv _ |- _] => destruct H
            | [H: p2st_decode_inv _ |- _] => destruct H
            | [H: p2st_stalled_inv _ |- _] => destruct H
-           | [H: p2st_raw_inv _ |- _] => destruct H
-           | [H: p2st_scoreboard_inv _ |- _] => destruct H
+           | [H: p2st_exec_inv _ |- _] => destruct H
+           | [H: p2st_epochs_inv _ |- _] => destruct H
+           | [H: p2st_pc_inv _ |- _] => destruct H
            end;
     kinv_red.
 
@@ -276,19 +462,102 @@ Section Invariants.
     try rewrite Hd2eOpType in *;
     try rewrite Hd2eDst in *;
     try rewrite Hd2eAddr in *;
-    try rewrite Hd2eVal in *;
+    try rewrite Hd2eVal1 in *;
+    try rewrite Hd2eVal2 in *;
     try rewrite Hd2eRawInst in *;
     try rewrite Hd2eCurPc in *;
     try rewrite Hd2eNextPc in *;
-    try rewrite Hd2eEpoch in *.
+    try rewrite Hd2eEpoch in *;
+    try rewrite He2wDecInst in *;
+    try rewrite He2wVal in *.
 
   Ltac p2st_inv_tac := p2st_inv_old; p2st_inv_new; d2e_abs_tac.
 
-  Lemma p2st_scoreboard_inv_ok':
+  Lemma p2st_epochs_inv_ok':
     forall init n ll,
       init = initRegs (getRegInits p2stInl) ->
       Multistep p2stInl init n ll ->
-      p2st_scoreboard_inv n.
+      p2st_epochs_inv n.
+  Proof. (* SKIP_PROOF_ON
+    induction 2; intros.
+
+    - p2st_inv_old.
+      unfold getRegInits, fst, p2stInl, ProcTwoStInl.p2stInl, projT1.
+      p2st_inv_new; simpl in *; kinv_simpl.
+
+    - kinvert.
+      + mred.
+      + mred.
+      + kinv_dest_custom p2st_inv_tac;
+          try (destruct x0, eepochv5; intuition idtac; fail).
+        * rewrite H14 in H4; exfalso; eapply negb_eq_false; eauto.
+      + kinv_dest_custom p2st_inv_tac; try reflexivity.
+      + kinv_dest_custom p2st_inv_tac; try reflexivity.
+      + kinv_dest_custom p2st_inv_tac; try reflexivity.
+      + kinv_dest_custom p2st_inv_tac; try reflexivity.
+      + kinv_dest_custom p2st_inv_tac.
+        * reflexivity.
+        * intuition idtac.
+        * intuition idtac.
+      + kinv_dest_custom p2st_inv_tac.
+        * reflexivity.
+        * intuition idtac.
+        * intuition idtac.
+      + kinv_dest_custom p2st_inv_tac.
+      + kinv_dest_custom p2st_inv_tac.
+      + kinv_dest_custom p2st_inv_tac.
+        rewrite H4 in H2; exfalso; eapply negb_eq_false; eauto.
+      + kinv_dest_custom p2st_inv_tac.
+      + kinv_dest_custom p2st_inv_tac.
+      + kinv_dest_custom p2st_inv_tac.
+      + kinv_dest_custom p2st_inv_tac.
+        rewrite H4 in H2; exfalso; eapply negb_eq_false; eauto.
+      + kinv_dest_custom p2st_inv_tac.
+        rewrite H4 in H2; exfalso; eapply negb_eq_false; eauto.
+
+        END_SKIP_PROOF_ON *) admit.
+  Qed.
+
+  Lemma p2st_pc_inv_ok':
+    forall init n ll,
+      init = initRegs (getRegInits p2stInl) ->
+      Multistep p2stInl init n ll ->
+      p2st_pc_inv n.
+  Proof. (* SKIP_PROOF_ON
+    induction 2; intros.
+
+    - p2st_inv_old.
+      unfold getRegInits, fst, p2stInl, ProcTwoStInl.p2stInl, projT1.
+      p2st_inv_new; simpl in *; kinv_simpl.
+
+    - pose proof (p2st_epochs_inv_ok' H H0).
+      kinvert.
+      + mred.
+      + mred.
+      + kinv_dest_custom p2st_inv_tac.
+      + kinv_dest_custom p2st_inv_tac; intuition idtac.
+      + kinv_dest_custom p2st_inv_tac; intuition idtac.
+      + kinv_dest_custom p2st_inv_tac; intuition idtac.
+      + kinv_dest_custom p2st_inv_tac; intuition idtac.
+      + kinv_dest_custom p2st_inv_tac; intuition idtac.
+      + kinv_dest_custom p2st_inv_tac; intuition idtac.
+      + kinv_dest_custom p2st_inv_tac.
+      + kinv_dest_custom p2st_inv_tac; rewrite H10 in H8; intuition idtac.
+      + kinv_dest_custom p2st_inv_tac.
+      + kinv_dest_custom p2st_inv_tac; rewrite H10 in H8; intuition idtac.
+      + kinv_dest_custom p2st_inv_tac.
+      + kinv_dest_custom p2st_inv_tac.
+      + kinv_dest_custom p2st_inv_tac.
+      + kinv_dest_custom p2st_inv_tac.
+
+        END_SKIP_PROOF_ON *) admit.
+  Qed.
+
+  Lemma p2st_scoreboard_waw_inv_ok':
+    forall init n ll,
+      init = initRegs (getRegInits p2stInl) ->
+      Multistep p2stInl init n ll ->
+      p2st_scoreboard_waw_inv n.
   Proof. (* SKIP_PROOF_ON
     induction 2.
 
@@ -300,25 +569,30 @@ Section Invariants.
       + mred.
       + mred.
       + kinv_dest_custom p2st_inv_tac.
+      + kinv_dest_custom p2st_inv_tac; try (find_if_inside; intuition idtac; fail);
+          try (simpl in H7; rewrite H7 in H10; rewrite H10 in H9; inv H9; fail);
+          try (simpl in H7; rewrite H7 in H10; rewrite H10 in H6; inv H6; fail).
+      + kinv_dest_custom p2st_inv_tac; try (rewrite e in H2; inv H2; fail);
+          try (rewrite e in H8; inv H8; fail).
+      + kinv_dest_custom p2st_inv_tac; try (rewrite e in H2; inv H2; fail);
+          try (rewrite e in H7; inv H7; fail).
+      + kinv_dest_custom p2st_inv_tac; try (find_if_inside; intuition idtac; fail);
+          try (simpl in H7; rewrite H7 in H10; rewrite H10 in H9; inv H9; fail);
+          try (simpl in H7; rewrite H7 in H10; rewrite H10 in H6; inv H6; fail).
+      + kinv_dest_custom p2st_inv_tac; intuition idtac.
+      + kinv_dest_custom p2st_inv_tac; intuition idtac.
       + kinv_dest_custom p2st_inv_tac.
       + kinv_dest_custom p2st_inv_tac.
       + kinv_dest_custom p2st_inv_tac.
       + kinv_dest_custom p2st_inv_tac.
+      + kinv_dest_custom p2st_inv_tac; try (find_if_inside; intuition idtac; fail).
       + kinv_dest_custom p2st_inv_tac.
       + kinv_dest_custom p2st_inv_tac.
-      + kinv_dest_custom p2st_inv_tac.
-      + kinv_dest_custom p2st_inv_tac;
-          try (match goal with
-               | [H1: ?x ?s1 = _, H2: ?x ?s2 = _ |- _] => change s1 with s2 in H1
-               end; rewrite e in H2; inv H2).
-      + kinv_dest_custom p2st_inv_tac.
-      + kinv_dest_custom p2st_inv_tac.
-      + kinv_dest_custom p2st_inv_tac.
-      + kinv_dest_custom p2st_inv_tac.
+      + kinv_dest_custom p2st_inv_tac; try (find_if_inside; intuition idtac; fail).
 
         END_SKIP_PROOF_ON *) admit.
   Qed.
-
+  
   Lemma p2st_raw_inv_ok':
     forall init n ll,
       init = initRegs (getRegInits p2stInl) ->
@@ -331,19 +605,49 @@ Section Invariants.
       unfold getRegInits, fst, p2stInl, ProcTwoStInl.p2stInl, projT1.
       p2st_inv_new; simpl in *; kinv_simpl.
 
-    - pose proof (p2st_scoreboard_inv_ok' H H0).
-      kinvert.
+    - pose proof (p2st_scoreboard_waw_inv_ok' H H0).
+      kinvert.      
       + mred.
       + mred.
       + kinv_dest_custom p2st_inv_tac.
-      + kinv_dest_custom p2st_inv_tac; try (rewrite e in H5; inv H5; fail).
-        rewrite andb_true_l in H14; kinv_simpl; intuition idtac.
-      + kinv_dest_custom p2st_inv_tac; try (rewrite e in H7; inv H7; fail).
-        * rewrite andb_true_l in H4; kinv_simpl; intuition idtac.
-        * rewrite andb_true_l in H11; kinv_simpl; intuition idtac.
-      + kinv_dest_custom p2st_inv_tac; try (rewrite e in H5; inv H5; fail).
-        rewrite andb_true_l in H14; kinv_simpl; intuition idtac.
-      + kinv_dest_custom p2st_inv_tac; try (rewrite e in H7; inv H7; fail).
+      + kinv_dest_custom p2st_inv_tac; try (rewrite e in H7; inv H7; fail);
+          try (rewrite e in H8; inv H8; fail);
+          try (rewrite e in H9; inv H9; fail).
+        * simpl in H9; rewrite H9 in H3; unfold LdSrcK in *; rewrite H3 in H4; inv H4.
+        * simpl in H9; rewrite H9 in H3; unfold LdSrcK in *; rewrite H3 in H4; inv H4.
+        * simpl in H12; rewrite H12 in H10; unfold LdSrcK in *; rewrite H10 in H4; inv H4.
+        * simpl in H12; rewrite H12 in H10; unfold LdSrcK in *; rewrite H10 in H4; inv H4.
+      + kinv_dest_custom p2st_inv_tac; try (rewrite e in H7; inv H7; fail);
+          try (rewrite e in H8; inv H8; fail);
+          try (rewrite e in H9; inv H9; fail).
+        * simpl in H9; rewrite H9 in H3; unfold StSrcK in *; rewrite H3 in H4; inv H4.
+        * simpl in H9; rewrite H9 in H3; unfold StVSrcK in *; rewrite H3 in H11; inv H11.
+        * simpl in H9; rewrite H9 in H3; unfold StSrcK in *; rewrite H3 in H4; inv H4.
+        * simpl in H9; rewrite H9 in H3; unfold StVSrcK in *; rewrite H3 in H11; inv H11.
+        * simpl in H12; rewrite H12 in H10; unfold StSrcK in *; rewrite H10 in H4; inv H4.
+        * simpl in H12; rewrite H12 in H10; unfold StVSrcK in *; rewrite H10 in H11; inv H11.
+        * simpl in H12; rewrite H12 in H10; unfold StSrcK in *; rewrite H10 in H4; inv H4.
+        * simpl in H12; rewrite H12 in H10; unfold StVSrcK in *; rewrite H10 in H11; inv H11.
+      + kinv_dest_custom p2st_inv_tac; try (rewrite e in H7; inv H7; fail);
+          try (rewrite e in H4; inv H4; fail);
+          try (rewrite e in H8; inv H8; fail).
+        * simpl in H9; rewrite H9 in H3; unfold Src1K in *; rewrite H3 in H13; inv H13.
+        * simpl in H9; rewrite H9 in H3; unfold Src1K in *; rewrite H3 in H13; inv H13.
+        * simpl in H10; rewrite H10 in H9; unfold Src1K in *; rewrite H9 in H13; inv H13.
+        * simpl in H10; rewrite H10 in H9; unfold Src1K in *; rewrite H9 in H13; inv H13.
+      + kinv_dest_custom p2st_inv_tac; try (rewrite e in H7; inv H7; fail);
+          try (rewrite e in H8; inv H8; fail);
+          try (rewrite e in H9; inv H9; fail).
+        * simpl in H9; rewrite H9 in H3; unfold Src1K in *; rewrite H3 in H4; inv H4.
+        * simpl in H9; rewrite H9 in H3; unfold Src2K in *; rewrite H3 in H15; inv H15.
+        * simpl in H9; rewrite H9 in H3; unfold Src1K in *; rewrite H3 in H4; inv H4.
+        * simpl in H9; rewrite H9 in H3; unfold Src2K in *; rewrite H3 in H15; inv H15.
+        * simpl in H12; rewrite H12 in H10; unfold Src1K in *; rewrite H10 in H4; inv H4.
+        * simpl in H12; rewrite H12 in H10; unfold Src2K in *; rewrite H10 in H15; inv H15.
+        * simpl in H12; rewrite H12 in H10; unfold Src1K in *; rewrite H10 in H4; inv H4.
+        * simpl in H12; rewrite H12 in H10; unfold Src2K in *; rewrite H10 in H15; inv H15.
+      + kinv_dest_custom p2st_inv_tac; intuition idtac.
+      + kinv_dest_custom p2st_inv_tac; intuition idtac.
       + kinv_dest_custom p2st_inv_tac.
       + kinv_dest_custom p2st_inv_tac.
       + kinv_dest_custom p2st_inv_tac.
@@ -377,26 +681,22 @@ Section Invariants.
       + kinv_dest_custom p2st_inv_tac; try reflexivity; try (rewrite e in H1; inv H1; fail).
       + kinv_dest_custom p2st_inv_tac; try reflexivity; try (rewrite e in H1; inv H1; fail).
       + kinv_dest_custom p2st_inv_tac; try reflexivity; try (rewrite e in H1; inv H1; fail).
+      + kinv_dest_custom p2st_inv_tac; try (simpl; intuition idtac).
+      + kinv_dest_custom p2st_inv_tac; try (simpl; intuition idtac).
       + kinv_dest_custom p2st_inv_tac.
       + kinv_dest_custom p2st_inv_tac.
       + kinv_dest_custom p2st_inv_tac.
       + kinv_dest_custom p2st_inv_tac.
-      + kinv_dest_custom p2st_inv_tac.
-        * find_if_inside; [elim H15; auto|auto].
-        * find_if_inside; [elim H9; auto|auto].
-        * find_if_inside; [elim H17; auto|auto].
-        * find_if_inside; [elim H7; auto|auto].
-        * find_if_inside; [elim H15; auto|auto].
-        * find_if_inside; [elim H9; auto|auto].
-        * find_if_inside; [elim H17; auto|auto].
-        * find_if_inside; [elim H7; auto|auto].
+      + kinv_dest_custom p2st_inv_tac;
+          try (find_if_inside; [exfalso; intuition auto|intuition idtac]; fail).
       + kinv_dest_custom p2st_inv_tac.
       + kinv_dest_custom p2st_inv_tac.
-      + kinv_dest_custom p2st_inv_tac.
+      + kinv_dest_custom p2st_inv_tac;
+          try (find_if_inside; [exfalso; intuition auto|intuition idtac]; fail).
 
         END_SKIP_PROOF_ON *) admit.
   Qed.
-
+  
   Lemma p2st_stalled_inv_ok':
     forall init n ll,
       init = initRegs (getRegInits p2stInl) ->
@@ -426,15 +726,17 @@ Section Invariants.
       + kinv_dest_custom p2st_inv_tac.
       + kinv_dest_custom p2st_inv_tac.
       + kinv_dest_custom p2st_inv_tac.
+      + kinv_dest_custom p2st_inv_tac.
+      + kinv_dest_custom p2st_inv_tac.
 
         END_SKIP_PROOF_ON *) admit.
   Qed.
 
-  Lemma p2st_pc_epochs_inv_ok':
+  Lemma p2st_exec_inv_ok':
     forall init n ll,
       init = initRegs (getRegInits p2stInl) ->
       Multistep p2stInl init n ll ->
-      p2st_pc_epochs_inv n.
+      p2st_exec_inv n.
   Proof. (* SKIP_PROOF_ON
     induction 2; intros.
 
@@ -442,24 +744,34 @@ Section Invariants.
       unfold getRegInits, fst, p2stInl, ProcTwoStInl.p2stInl, projT1.
       p2st_inv_new; simpl in *; kinv_simpl.
 
-    - kinvert.
+    - pose proof (p2st_decode_inv_ok' H H0).
+      pose proof (p2st_raw_inv_ok' H H0).
+      kinvert.
       + mred.
       + mred.
       + kinv_dest_custom p2st_inv_tac.
-        * destruct x0, eepochv0; intuition idtac.
-        * destruct x0, eepochv0; intuition idtac.
-      + kinv_dest_custom p2st_inv_tac; try reflexivity.
-      + kinv_dest_custom p2st_inv_tac; try reflexivity.
-      + kinv_dest_custom p2st_inv_tac; try reflexivity.
-      + kinv_dest_custom p2st_inv_tac; try reflexivity.
-      + kinv_dest_custom p2st_inv_tac.
-      + kinv_dest_custom p2st_inv_tac; intuition idtac.
-      + kinv_dest_custom p2st_inv_tac.
-      + kinv_dest_custom p2st_inv_tac; intuition idtac.
       + kinv_dest_custom p2st_inv_tac.
       + kinv_dest_custom p2st_inv_tac.
       + kinv_dest_custom p2st_inv_tac.
       + kinv_dest_custom p2st_inv_tac.
+      + kinv_dest_custom p2st_inv_tac.
+        simpl; rewrite <-H6, <-H12; reflexivity.
+      + kinv_dest_custom p2st_inv_tac.
+        elim n0; assumption.
+      + kinv_dest_custom p2st_inv_tac.
+      + kinv_dest_custom p2st_inv_tac.
+      + kinv_dest_custom p2st_inv_tac.
+      + kinv_dest_custom p2st_inv_tac.
+      + kinv_dest_custom p2st_inv_tac;
+          try (find_if_inside; [elim H21; auto|];
+               find_if_inside; [elim H22; auto|];
+               intuition idtac; fail).
+      + kinv_dest_custom p2st_inv_tac.
+      + kinv_dest_custom p2st_inv_tac.
+      + kinv_dest_custom p2st_inv_tac;
+          try (find_if_inside; [elim H21; auto|];
+               find_if_inside; [elim H22; auto|];
+               intuition idtac; fail).
 
         END_SKIP_PROOF_ON *) admit.
   Qed.
@@ -467,20 +779,25 @@ Section Invariants.
   Lemma p2st_inv_ok:
     forall o,
       reachable o p2stInl ->
-      p2st_pc_epochs_inv o /\ p2st_decode_inv o /\ p2st_stalled_inv o /\
-      p2st_raw_inv o /\ p2st_scoreboard_inv o.
+      p2st_scoreboard_waw_inv o /\ p2st_raw_inv o /\ p2st_decode_inv o /\
+      p2st_stalled_inv o /\ p2st_exec_inv o /\ p2st_epochs_inv o /\ p2st_pc_inv o.
   Proof.
     intros; inv H; inv H0.
     repeat split.
-    - eapply p2st_pc_epochs_inv_ok'; eauto.
+    - eapply p2st_scoreboard_waw_inv_ok'; eauto.
+    - eapply p2st_raw_inv_ok'; eauto.
     - eapply p2st_decode_inv_ok'; eauto.
     - eapply p2st_stalled_inv_ok'; eauto.
-    - eapply p2st_raw_inv_ok'; eauto.
-    - eapply p2st_scoreboard_inv_ok'; eauto.
+    - eapply p2st_exec_inv_ok'; eauto.
+    - eapply p2st_epochs_inv_ok'; eauto.
+    - eapply p2st_pc_inv_ok'; eauto.
   Qed.
 
 End Invariants.
 
-Hint Unfold p2st_pc_epochs_inv_body p2st_decode_inv_body p2st_stalled_inv_body
-     p2st_raw_inv_body p2st_scoreboard_inv_body : InvDefs.
+Hint Unfold p2st_scoreboard_waw_inv_body p2st_raw_inv_body
+     p2st_decode_inv_body p2st_stalled_inv_body
+     p2st_exec_inv_body p2st_epochs_inv_body p2st_pc_inv_body : InvDefs.
+
+Close Scope fmap.
 
