examples/ProcFDInv.v
@@ -36,7 +36,8 @@ Section Invariants.
                 Expr ty (SyntaxKind (Bit 2)) -> (* opTy *)
                 Expr ty (SyntaxKind (Bit rfIdx)) -> (* dst *)
                 Expr ty (SyntaxKind (Bit addrSize)) -> (* addr *)
-                Expr ty (SyntaxKind (Data lgDataBytes)) -> (* val *)
+                Expr ty (SyntaxKind (Data lgDataBytes)) -> (* val1 *)
+                Expr ty (SyntaxKind (Data lgDataBytes)) -> (* val2 *)
                 Expr ty (SyntaxKind (Data lgDataBytes)) -> (* rawInst *)
                 Expr ty (SyntaxKind (Bit addrSize)) -> (* curPc *)
                 Expr ty (SyntaxKind (Bit addrSize)) -> (* nextPc *)
@@ -77,7 +78,7 @@ Section Invariants.
   Definition fetchDecodeInl := projT1 (fetchDecodeInl
                                          getOptype getLdDst getLdAddr getLdSrc calcLdAddr
                                          getStAddr getStSrc calcStAddr getStVSrc
-                                         getSrc1 predictNextPc
+                                         getSrc1 getSrc2 getDst predictNextPc
                                          d2ePack f2dPack f2dRawInst f2dCurPc f2dNextPc f2dEpoch).
 
   Definition fetchDecode_inv_body
